iris/ProofUserinit.v
@@ -773,7 +773,7 @@ Section ProofUserinit.
     iAssert (∀ W : uvis, uslot W)%I as "Hjslot".
     { iPoseProof UG.uexec_wp_gen as "#Hgen".
       iIntros (W). iApply (UexecCond.cond_entry_slot W with "Hgen"). }
-    iMod (park_token_park N rest (MkUstate (upd_cwd V ipv) M) Hwf Hrest
+    iMod (park_token_park N rest (MkUstate (upd_cwd V ipv) M) fdt0 Hwf Hrest
             with "Htoken Htext Hwire Htramp Hmk Hstack Henv Hown Hfrag Hjslot
                   [Hks Hctx Hpriv Hfd Hirs]")
       as "Hpctx".
